Semantics.v
@@ -21,7 +21,7 @@ Set Asymmetric Patterns.
 Reserved Notation " x '~~>' y " (at level 50, left associativity).
 
 Inductive rstep : config -> config -> Prop :=
-| RStepGetfield1 : forall P H S e f Y s c C o cl1 cl2 H' S',
+| RStepGetfield1 : forall P H H' Σ' Σ e f Y s c C o σ1' σ2',
   e = s_expr_getfield (s_expr_val (s_val_ref_c Y)) f ->
   Y = s_ref_c_symb s ->
   unresolved H s ->
@@ -29,11 +29,11 @@ Inductive rstep : config -> config -> Prop :=
   c = class_name C ->
   new_obj_symb P c o ->
   H' = add_obj_symb H s o -> 
-  cl1 = s_val_not (s_val_eq (s_val_ref_c Y) (s_val_ref_c s_ref_c_null)) -> (* TODO redundant? *)
-  cl2 = s_val_subtype (s_val_ref_c Y) (s_ty_class c) ->
-  S' = S ++ [cl1 ; cl2] ->
-  (P, H, S, e) ~~> (P, H', S', e)
-| RStepGetfield2 : forall P H S e f Y s c c' C' o o' cl H' S',
+  σ1' = s_val_not (s_val_eq (s_val_ref_c Y) (s_val_ref_c s_ref_c_null)) -> (* TODO redundant? *)
+  σ2' = s_val_subtype (s_val_ref_c Y) (s_ty_class c) ->
+  Σ' = Σ ++ [σ1' ; σ2'] ->
+  (P, H, Σ, e) ~~> (P, H', Σ', e)
+| RStepGetfield2 : forall P H H' Σ Σ' e f Y s c c' C' o o' σ',
   e = s_expr_getfield (s_expr_val (s_val_ref_c Y)) f ->
   Y = s_ref_c_symb s ->
   has_obj H Y o ->
@@ -43,10 +43,10 @@ Inductive rstep : config -> config -> Prop :=
   c' = class_name C' ->
   refine_obj_symb P c c' o o' ->
   H' = repl_obj H Y o' ->
-  cl = s_val_subtype (s_val_ref_c Y) (s_ty_class c') ->
-  S' = S ++ [cl] ->
-  (P, H, S, e) ~~> (P, H', S', e)
-| RStepGetfield3 : forall P H S S' e f C t Y Z s s' o o' σ cl H',
+  σ' = s_val_subtype (s_val_ref_c Y) (s_ty_class c') ->
+  Σ' = Σ ++ [σ'] ->
+  (P, H, Σ, e) ~~> (P, H', Σ', e)
+| RStepGetfield3 : forall P H H' Σ Σ' e f C t Y Z s s' o o' σ σ',
   e = s_expr_getfield (s_expr_val (s_val_ref_c Y)) f ->
   Y = s_ref_c_symb s ->
   has_obj H Y o ->
@@ -58,10 +58,10 @@ Inductive rstep : config -> config -> Prop :=
   Z = s_prim_c_symb s' ->
   o' = upd_obj o f σ ->
   H' = repl_obj H Y o' ->
-  cl = s_val_field s f s' ->
-  S' = S ++ [cl] ->
-  (P, H, S, e) ~~> (P, H', S', e)
-| RStepGetfield4 : forall P H S S' e f C t Y Z s s' o o' σ cl H',
+  σ' = s_val_field s f s' ->
+  Σ' = Σ ++ [σ'] ->
+  (P, H, Σ, e) ~~> (P, H', Σ', e)
+| RStepGetfield4 : forall P H H' Σ Σ' e f C t Y Z s s' o o' σ σ',
   e = s_expr_getfield (s_expr_val (s_val_ref_c Y)) f ->
   Y = s_ref_c_symb s ->
   has_obj H Y o ->
@@ -73,10 +73,10 @@ Inductive rstep : config -> config -> Prop :=
   Z = s_ref_c_symb s' ->
   o' = upd_obj o f σ ->
   H' = repl_obj H Y o' ->
-  cl = s_val_field s f s' ->
-  S' = S ++ [cl] ->
-  (P, H, S, e) ~~> (P, H', S', e)
-| RStepPutfield1 : forall P H S e f Y σ s c C o cl1 cl2 H' S',
+  σ' = s_val_field s f s' ->
+  Σ' = Σ ++ [σ'] ->
+  (P, H, Σ, e) ~~> (P, H', Σ', e)
+| RStepPutfield1 : forall P H H' Σ Σ' e f Y σ s c C o σ1' σ2',
   e = s_expr_putfield (s_expr_val (s_val_ref_c Y)) f (s_expr_val σ) ->
   Y = s_ref_c_symb s ->
   unresolved H s ->
@@ -84,11 +84,11 @@ Inductive rstep : config -> config -> Prop :=
   c = class_name C ->
   new_obj_symb P c o ->
   H' = add_obj_symb H s o ->
-  cl1 = s_val_not (s_val_eq (s_val_ref_c Y) (s_val_ref_c s_ref_c_null)) -> (* TODO redundant? *)
-  cl2 = s_val_subtype (s_val_ref_c Y) (s_ty_class c) ->
-  S' = S ++ [cl1 ; cl2] ->
-  (P, H, S, e) ~~> (P, H', S', e)
-| RStepPutfield2 : forall P H S e f Y σ s c c' C' o o' cl H' S',
+  σ1' = s_val_not (s_val_eq (s_val_ref_c Y) (s_val_ref_c s_ref_c_null)) -> (* TODO redundant? *)
+  σ2' = s_val_subtype (s_val_ref_c Y) (s_ty_class c) ->
+  Σ' = Σ ++ [σ1' ; σ2'] ->
+  (P, H, Σ, e) ~~> (P, H', Σ', e)
+| RStepPutfield2 : forall P H H' Σ Σ' e f Y σ σ' s c c' C' o o',
   e = s_expr_putfield (s_expr_val (s_val_ref_c Y)) f (s_expr_val σ) ->
   Y = s_ref_c_symb s ->
   has_obj H Y o ->
@@ -98,51 +98,51 @@ Inductive rstep : config -> config -> Prop :=
   c' = class_name C' ->
   refine_obj_symb P c c' o o' ->
   H' = repl_obj H Y o' ->
-  cl = s_val_subtype (s_val_ref_c Y) (s_ty_class c') ->
-  S' = S ++ [cl] ->
-  (P, H, S, e) ~~> (P, H', S', e)
-| RStepCtxGetfield : forall P H H' S S' e e' f,
-  (P, H, S, e) ~~> (P, H', S', e') ->  
-  (P, H, S, s_expr_getfield e f) ~~> (P, H', S', s_expr_getfield e' f)
-| RStepCtxPutfield1 : forall P H H' S S' e e' e1 f,
-  (P, H, S, e) ~~> (P, H', S', e') ->  
-  (P, H, S, s_expr_putfield e f e1) ~~> (P, H', S', s_expr_putfield e' f e1)
-| RStepCtxPutfield2 : forall P H H' S S' e e' σ f,
-  (P, H, S, e) ~~> (P, H', S', e') ->  
-  (P, H, S, s_expr_putfield (s_expr_val σ) f e) ~~> (P, H', S', s_expr_putfield (s_expr_val σ) f e')
-| RStepCtxLet : forall P H H' S S' e e' e1 x,
-  (P, H, S, e) ~~> (P, H', S', e') ->  
-  (P, H, S, s_expr_let x e e1) ~~> (P, H', S', s_expr_let x e' e1)
-| RStepCtxAdd1 : forall P H H' S S' e e' e1,
-  (P, H, S, e) ~~> (P, H', S', e') ->  
-  (P, H, S, s_expr_add e e1) ~~> (P, H', S', s_expr_add e' e1)
-| RStepCtxAdd2 : forall P H H' S S' e e' σ,
-  (P, H, S, e) ~~> (P, H', S', e') ->  
-  (P, H, S, s_expr_add (s_expr_val σ) e) ~~> (P, H', S', s_expr_add (s_expr_val σ) e')
-| RStepCtxLt1 : forall P H H' S S' e e' e1,
-  (P, H, S, e) ~~> (P, H', S', e') ->
-  (P, H, S, s_expr_lt e e1) ~~> (P, H', S', s_expr_lt e' e1)
-| RStepCtxLt2 : forall P H H' S S' e e' σ,
-  (P, H, S, e) ~~> (P, H', S', e') ->
-  (P, H, S, s_expr_lt (s_expr_val σ) e) ~~> (P, H', S', s_expr_lt (s_expr_val σ) e')
-| RStepCtxEq1 : forall P H H' S S' e e' e1,
-  (P, H, S, e) ~~> (P, H', S', e') ->  
-  (P, H, S, s_expr_eq e e1) ~~> (P, H', S', s_expr_eq e' e1)
-| RStepCtxEq2 : forall P H H' S S' e e' σ,
-  (P, H, S, e) ~~> (P, H', S', e') ->  
-  (P, H, S, s_expr_eq (s_expr_val σ) e) ~~> (P, H', S', s_expr_eq (s_expr_val σ) e')
-| RStepCtxInstanceof : forall P H H' S S' e e' c,
-  (P, H, S, e) ~~> (P, H', S', e') ->  
-  (P, H, S, s_expr_instanceof e c) ~~> (P, H', S', s_expr_instanceof e' c)
-| RStepCtxIf : forall P H H' S S' e e' e1 e2,
-  (P, H, S, e) ~~> (P, H', S', e') ->  
-  (P, H, S, s_expr_if e e1 e2) ~~> (P, H', S', s_expr_if e' e1 e2)
-| RStepCtxInvoke1 : forall P H H' S S' e e' e1 m,
-  (P, H, S, e) ~~> (P, H', S', e') ->  
-  (P, H, S, s_expr_invoke e m e1) ~~> (P, H', S', s_expr_invoke e' m e1)
-| RStepCtxInvoke2 : forall P H H' S S' e e' σ m,
-  (P, H, S, e) ~~> (P, H', S', e') ->  
-  (P, H, S, s_expr_invoke (s_expr_val σ) m e) ~~> (P, H', S', s_expr_invoke (s_expr_val σ) m e')
+  σ' = s_val_subtype (s_val_ref_c Y) (s_ty_class c') ->
+  Σ' = Σ ++ [σ'] ->
+  (P, H, Σ, e) ~~> (P, H', Σ', e)
+| RStepCtxGetfield : forall P H H' Σ Σ' e e' f,
+  (P, H, Σ, e) ~~> (P, H', Σ', e') ->  
+  (P, H, Σ, s_expr_getfield e f) ~~> (P, H', Σ', s_expr_getfield e' f)
+| RStepCtxPutfield1 : forall P H H' Σ Σ' e e' e1 f,
+  (P, H, Σ, e) ~~> (P, H', Σ', e') ->  
+  (P, H, Σ, s_expr_putfield e f e1) ~~> (P, H', Σ', s_expr_putfield e' f e1)
+| RStepCtxPutfield2 : forall P H H' Σ Σ' e e' σ f,
+  (P, H, Σ, e) ~~> (P, H', Σ', e') ->  
+  (P, H, Σ, s_expr_putfield (s_expr_val σ) f e) ~~> (P, H', Σ', s_expr_putfield (s_expr_val σ) f e')
+| RStepCtxLet : forall P H H' Σ Σ' e e' e1 x,
+  (P, H, Σ, e) ~~> (P, H', Σ', e') ->  
+  (P, H, Σ, s_expr_let x e e1) ~~> (P, H', Σ', s_expr_let x e' e1)
+| RStepCtxAdd1 : forall P H H' Σ Σ' e e' e1,
+  (P, H, Σ, e) ~~> (P, H', Σ', e') ->  
+  (P, H, Σ, s_expr_add e e1) ~~> (P, H', Σ', s_expr_add e' e1)
+| RStepCtxAdd2 : forall P H H' Σ Σ' e e' σ,
+  (P, H, Σ, e) ~~> (P, H', Σ', e') ->  
+  (P, H, Σ, s_expr_add (s_expr_val σ) e) ~~> (P, H', Σ', s_expr_add (s_expr_val σ) e')
+| RStepCtxLt1 : forall P H H' Σ Σ' e e' e1,
+  (P, H, Σ, e) ~~> (P, H', Σ', e') ->
+  (P, H, Σ, s_expr_lt e e1) ~~> (P, H', Σ', s_expr_lt e' e1)
+| RStepCtxLt2 : forall P H H' Σ Σ' e e' σ,
+  (P, H, Σ, e) ~~> (P, H', Σ', e') ->
+  (P, H, Σ, s_expr_lt (s_expr_val σ) e) ~~> (P, H', Σ', s_expr_lt (s_expr_val σ) e')
+| RStepCtxEq1 : forall P H H' Σ Σ' e e' e1,
+  (P, H, Σ, e) ~~> (P, H', Σ', e') ->  
+  (P, H, Σ, s_expr_eq e e1) ~~> (P, H', Σ', s_expr_eq e' e1)
+| RStepCtxEq2 : forall P H H' Σ Σ' e e' σ,
+  (P, H, Σ, e) ~~> (P, H', Σ', e') ->  
+  (P, H, Σ, s_expr_eq (s_expr_val σ) e) ~~> (P, H', Σ', s_expr_eq (s_expr_val σ) e')
+| RStepCtxInstanceof : forall P H H' Σ Σ' e e' c,
+  (P, H, Σ, e) ~~> (P, H', Σ', e') ->  
+  (P, H, Σ, s_expr_instanceof e c) ~~> (P, H', Σ', s_expr_instanceof e' c)
+| RStepCtxIf : forall P H H' Σ Σ' e e' e1 e2,
+  (P, H, Σ, e) ~~> (P, H', Σ', e') ->  
+  (P, H, Σ, s_expr_if e e1 e2) ~~> (P, H', Σ', s_expr_if e' e1 e2)
+| RStepCtxInvoke1 : forall P H H' Σ Σ' e e' e1 m,
+  (P, H, Σ, e) ~~> (P, H', Σ', e') ->  
+  (P, H, Σ, s_expr_invoke e m e1) ~~> (P, H', Σ', s_expr_invoke e' m e1)
+| RStepCtxInvoke2 : forall P H H' Σ Σ' e e' σ m,
+  (P, H, Σ, e) ~~> (P, H', Σ', e') ->  
+  (P, H, Σ, s_expr_invoke (s_expr_val σ) m e) ~~> (P, H', Σ', s_expr_invoke (s_expr_val σ) m e')
 where " x '~~>' y " := (rstep x y).
 
 (* Reflexive-transitive closure of the refinement 
@@ -162,43 +162,44 @@ Reserved Notation " x '-->' y " (at level 50, left associativity).
 Reserved Notation " x '==>' y " (at level 50, left associativity).
 
 Inductive cstep : config -> config -> Prop :=
-| CStepNew : forall P H S e c C o u H' e',
+| CStepNew : forall P H H' Σ e e' c C o u,
   e = s_expr_new c -> 
   cdecl P c = Some C ->
   new_obj P c o ->
   (H', u) = add_obj H o ->
   e' = s_expr_val (s_val_ref_c u) ->
-  (P, H, S, e) --> (P, H', S, e')
-| CStepGetfield1 : forall P H S e f l n o σ e',
+  (P, H, Σ, e) --> (P, H', Σ, e')
+| CStepGetfield1 : forall P H Σ e e' f l n o σ,
   e = s_expr_getfield (s_expr_val (s_val_ref_c l)) f ->
   l = s_ref_c_loc (s_loc_l n) ->
   has_obj H l o ->
   get o f = Some σ ->
   e' = s_expr_val σ ->
-  (P, H, S, e) --> (P, H, S, e')
-| CStepGetfield2 : forall P H S e f Y s o σ e',
+  (P, H, Σ, e) --> (P, H, Σ, e')
+| CStepGetfield2 : forall P H Σ e e' f Y s o σ,
   e = s_expr_getfield (s_expr_val (s_val_ref_c Y)) f ->
   Y = s_ref_c_symb s ->
   has_obj H Y o ->
   get o f = Some σ ->
   ~(σ = s_val_unassumed) ->
   e' = s_expr_val σ ->
-  (P, H, S, e) --> (P, H, S, e')
-| CStepGetfield3 : forall P H S e σ f H1' S1' σ1 σ2 σ1' σ2' H' S' e',
-  (P, H, S, (s_expr_getfield (s_expr_val σ1) f)) ==> (P, H1', S1', (s_expr_val σ1')) ->
-  (P, H1', S1', (s_expr_getfield (s_expr_val σ2) f)) ==> (P, H', S', (s_expr_val σ2')) ->
+  (P, H, Σ, e) --> (P, H, Σ, e')
+| CStepGetfield3 : forall P H H' H1' Σ Σ' Σ1' Σ2' e e' f σ σ1 σ2 σ1' σ2',
+  (P, H, Σ, (s_expr_getfield (s_expr_val σ1) f)) ==> (P, H1', Σ1', (s_expr_val σ1')) ->
+  (P, H1', Σ, (s_expr_getfield (s_expr_val σ2) f)) ==> (P, H', Σ2', (s_expr_val σ2')) ->
+  Σ' = merge_pc σ Σ1' Σ2' ->
   e = s_expr_getfield (s_expr_val (s_val_ite σ σ1 σ2)) f ->
   e' = s_expr_val (s_val_ite σ σ1' σ2') ->
-  (P, H, S, e) --> (P, H', S', e')
-| CStepPutfield1 : forall P H S e e' σ f l n o o' H',
+  (P, H, Σ, e) --> (P, H', Σ', e')
+| CStepPutfield1 : forall P H H' Σ e e' σ f l n o o',
   e' = s_expr_val σ ->
   e = s_expr_putfield (s_expr_val (s_val_ref_c l)) f e' ->
   l = s_ref_c_loc (s_loc_l n) ->
   has_obj H l o ->
   o' = upd_obj o f σ ->
   H' = repl_obj H l o' ->
-  (P, H, S, e) --> (P, H', S, e')
-| CStepPutfield2 : forall P H S e e' σ σ' f Y s o o' HRefined H',
+  (P, H, Σ, e) --> (P, H', Σ, e')
+| CStepPutfield2 : forall P H HRefined H' Σ e e' σ σ' f Y s o o',
   e' = s_expr_val σ ->
   e = s_expr_putfield (s_expr_val (s_val_ref_c Y)) f e' ->
   Y = s_ref_c_symb s ->
@@ -207,155 +208,155 @@ Inductive cstep : config -> config -> Prop :=
   update f Y σ H HRefined ->
   o' = upd_obj o f σ ->
   H' = repl_obj HRefined Y o' ->
-  (P, H, S, e) --> (P, H', S, e')
-| CStepPutfield3 : forall P H S Setc e e' f σ H1' H2' S1' S2' σ1 σ2 σ' H' S',
+  (P, H, Σ, e) --> (P, H', Σ, e')
+| CStepPutfield3 : forall P H H' H1' H2' Σ Σ' Σ1' Σ2' Σetc e e' f σ σ1 σ2 σ',
   e' = s_expr_val σ' ->
-  (P, H, S, s_expr_putfield (s_expr_val σ1) f e') ==> (P, H1', S1', e') ->
-  (P, H, S, s_expr_putfield (s_expr_val σ2) f e') ==> (P, H2', S2', e') ->
+  (P, H, Σ, s_expr_putfield (s_expr_val σ1) f e') ==> (P, H1', Σ1', e') ->
+  (P, H, Σ, s_expr_putfield (s_expr_val σ2) f e') ==> (P, H2', Σ2', e') ->
   e = s_expr_putfield (s_expr_val (s_val_ite σ σ1 σ2)) f e' ->
   merge H1' H2' H' H f σ ->
-  merge_clauses H1' H2' f = Some Setc ->
-  S' = S1' ++ S2' ++ Setc ->
-  (P, H, S, e) --> (P, H', S', e')
-| CStepLet : forall P H S e x σ e1 e',
+  merge_clauses H1' H2' f = Some Σetc ->
+  Σ' = (merge_pc σ Σ1' Σ2') ++ Σetc ->
+  (P, H, Σ, e) --> (P, H', Σ', e')
+| CStepLet : forall P H Σ e e' e1 x σ,
   e = s_expr_let x (s_expr_val σ) e1 ->
   e' = repl_var e1 x (s_expr_val σ) ->
-  (P, H, S, e) --> (P, H, S, e')
-| CStepAdd1 : forall P H S e n1 n2 e',
+  (P, H, Σ, e) --> (P, H, Σ, e')
+| CStepAdd1 : forall P H Σ e e' n1 n2,
   e = s_expr_add (s_expr_val (s_val_prim_c (s_prim_c_int (s_int_l n1)))) (s_expr_val (s_val_prim_c (s_prim_c_int (s_int_l n2)))) ->
   e' = s_expr_val (s_val_prim_c (s_prim_c_int (s_int_l (n1 + n2)))) ->
-  (P, H, S, e) --> (P, H, S, e')
-| CStepAdd2 : forall P H S e e' n σ1 σ2,
+  (P, H, Σ, e) --> (P, H, Σ, e')
+| CStepAdd2 : forall P H Σ e e' n σ1 σ2,
   e = s_expr_add (s_expr_val σ1) (s_expr_val σ2) ->
   (σ1 <> s_val_prim_c (s_prim_c_int (s_int_l n)) \/ σ2 <> s_val_prim_c (s_prim_c_int (s_int_l n))) ->
   e' = s_expr_val (s_val_add σ1 σ2) ->
-  (P, H, S, e) --> (P, H, S, e')
-| CStepSub1 : forall P H S e n1 n2 e',
+  (P, H, Σ, e) --> (P, H, Σ, e')
+| CStepSub1 : forall P H Σ e e' n1 n2,
   e = s_expr_sub (s_expr_val (s_val_prim_c (s_prim_c_int (s_int_l n1)))) (s_expr_val (s_val_prim_c (s_prim_c_int (s_int_l n2)))) ->
   e' = s_expr_val (s_val_prim_c (s_prim_c_int (s_int_l (n1 - n2)))) ->
-  (P, H, S, e) --> (P, H, S, e')
-| CStepSub2 : forall P H S e e' n σ1 σ2,
+  (P, H, Σ, e) --> (P, H, Σ, e')
+| CStepSub2 : forall P H Σ e e' n σ1 σ2,
   e = s_expr_sub (s_expr_val σ1) (s_expr_val σ2) ->
   (σ1 <> s_val_prim_c (s_prim_c_int (s_int_l n)) \/ σ2 <> s_val_prim_c (s_prim_c_int (s_int_l n))) ->
   e' = s_expr_val (s_val_sub σ1 σ2) ->
-  (P, H, S, e) --> (P, H, S, e')
-| CStepLt1 : forall P H S e n1 n2 e',
+  (P, H, Σ, e) --> (P, H, Σ, e')
+| CStepLt1 : forall P H Σ e e' n1 n2,
   e = s_expr_lt (s_expr_val (s_val_prim_c (s_prim_c_int (s_int_l n1)))) (s_expr_val (s_val_prim_c (s_prim_c_int (s_int_l n2)))) ->
   e' = s_expr_val (s_val_prim_c (s_prim_c_bool (if Nat.ltb n1 n2 then s_bool_true else s_bool_false))) ->
-  (P, H, S, e) --> (P, H, S, e')
-| CStepLt2 : forall P H S e e' n σ1 σ2,
+  (P, H, Σ, e) --> (P, H, Σ, e')
+| CStepLt2 : forall P H Σ e e' n σ1 σ2,
   e = s_expr_lt (s_expr_val σ1) (s_expr_val σ2) ->
   (σ1 <> s_val_prim_c (s_prim_c_int (s_int_l n)) \/ σ2 <> s_val_prim_c (s_prim_c_int (s_int_l n))) ->
   e' = s_expr_val (s_val_lt σ1 σ2) ->
-  (P, H, S, e) --> (P, H, S, e')
-| CStepAnd1 : forall P H S e e',
+  (P, H, Σ, e) --> (P, H, Σ, e')
+| CStepAnd1 : forall P H Σ e e',
   e = s_expr_and (s_expr_val (s_val_prim_c (s_prim_c_bool s_bool_true))) (s_expr_val (s_val_prim_c (s_prim_c_bool s_bool_true))) ->
   e' = s_expr_val (s_val_prim_c (s_prim_c_bool s_bool_true)) ->
-  (P, H, S, e) --> (P, H, S, e')
-| CStepAnd2 : forall P H S e e',
+  (P, H, Σ, e) --> (P, H, Σ, e')
+| CStepAnd2 : forall P H Σ e e',
   e = s_expr_and (s_expr_val (s_val_prim_c (s_prim_c_bool s_bool_true))) (s_expr_val (s_val_prim_c (s_prim_c_bool s_bool_false))) ->
   e' = s_expr_val (s_val_prim_c (s_prim_c_bool s_bool_false)) ->
-  (P, H, S, e) --> (P, H, S, e')
-| CStepAnd3 : forall P H S e e',
+  (P, H, Σ, e) --> (P, H, Σ, e')
+| CStepAnd3 : forall P H Σ e e',
   e = s_expr_and (s_expr_val (s_val_prim_c (s_prim_c_bool s_bool_false))) (s_expr_val (s_val_prim_c (s_prim_c_bool s_bool_true))) ->
   e' = s_expr_val (s_val_prim_c (s_prim_c_bool s_bool_false)) ->
-  (P, H, S, e) --> (P, H, S, e')
-| CStepAnd4 : forall P H S e e',
+  (P, H, Σ, e) --> (P, H, Σ, e')
+| CStepAnd4 : forall P H Σ e e',
   e = s_expr_and (s_expr_val (s_val_prim_c (s_prim_c_bool s_bool_false))) (s_expr_val (s_val_prim_c (s_prim_c_bool s_bool_false))) ->
   e' = s_expr_val (s_val_prim_c (s_prim_c_bool s_bool_false)) ->
-  (P, H, S, e) --> (P, H, S, e')
-| CStepAnd5 : forall P H S e e' b σ1 σ2,
+  (P, H, Σ, e) --> (P, H, Σ, e')
+| CStepAnd5 : forall P H Σ e e' b σ1 σ2,
   e = s_expr_and (s_expr_val σ1) (s_expr_val σ2) ->
   (σ1 <> s_val_prim_c (s_prim_c_bool b) \/ σ2 <> s_val_prim_c (s_prim_c_bool b)) ->
   e' = s_expr_val (s_val_and σ1 σ2) ->
-  (P, H, S, e) --> (P, H, S, e')
-| CStepOr1 : forall P H S e e',
+  (P, H, Σ, e) --> (P, H, Σ, e')
+| CStepOr1 : forall P H Σ e e',
   e = s_expr_or (s_expr_val (s_val_prim_c (s_prim_c_bool s_bool_true))) (s_expr_val (s_val_prim_c (s_prim_c_bool s_bool_true))) ->
   e' = s_expr_val (s_val_prim_c (s_prim_c_bool s_bool_true)) ->
-  (P, H, S, e) --> (P, H, S, e')
-| CStepOr2 : forall P H S e e',
+  (P, H, Σ, e) --> (P, H, Σ, e')
+| CStepOr2 : forall P H Σ e e',
   e = s_expr_or (s_expr_val (s_val_prim_c (s_prim_c_bool s_bool_true))) (s_expr_val (s_val_prim_c (s_prim_c_bool s_bool_false))) ->
   e' = s_expr_val (s_val_prim_c (s_prim_c_bool s_bool_true)) ->
-  (P, H, S, e) --> (P, H, S, e')
-| CStepOr3 : forall P H S e e',
+  (P, H, Σ, e) --> (P, H, Σ, e')
+| CStepOr3 : forall P H Σ e e',
   e = s_expr_or (s_expr_val (s_val_prim_c (s_prim_c_bool s_bool_false))) (s_expr_val (s_val_prim_c (s_prim_c_bool s_bool_true))) ->
   e' = s_expr_val (s_val_prim_c (s_prim_c_bool s_bool_true)) ->
-  (P, H, S, e) --> (P, H, S, e')
-| CStepOr4 : forall P H S e e',
+  (P, H, Σ, e) --> (P, H, Σ, e')
+| CStepOr4 : forall P H Σ e e',
   e = s_expr_or (s_expr_val (s_val_prim_c (s_prim_c_bool s_bool_false))) (s_expr_val (s_val_prim_c (s_prim_c_bool s_bool_false))) ->
   e' = s_expr_val (s_val_prim_c (s_prim_c_bool s_bool_false)) ->
-  (P, H, S, e) --> (P, H, S, e')
-| CStepOr5 : forall P H S e e' b σ1 σ2,
+  (P, H, Σ, e) --> (P, H, Σ, e')
+| CStepOr5 : forall P H Σ e e' b σ1 σ2,
   e = s_expr_or (s_expr_val σ1) (s_expr_val σ2) ->
   (σ1 <> s_val_prim_c (s_prim_c_bool b) \/ σ2 <> s_val_prim_c (s_prim_c_bool b)) ->
   e' = s_expr_val (s_val_or σ1 σ2) ->
-  (P, H, S, e) --> (P, H, S, e')
-| CStepNot1 : forall P H S e e',
+  (P, H, Σ, e) --> (P, H, Σ, e')
+| CStepNot1 : forall P H Σ e e',
   e = s_expr_not (s_expr_val (s_val_prim_c (s_prim_c_bool s_bool_true))) ->
   e' = s_expr_val (s_val_prim_c (s_prim_c_bool s_bool_false)) ->
-  (P, H, S, e) --> (P, H, S, e')
-| CStepNot2 : forall P H S e e',
+  (P, H, Σ, e) --> (P, H, Σ, e')
+| CStepNot2 : forall P H Σ e e',
   e = s_expr_not (s_expr_val (s_val_prim_c (s_prim_c_bool s_bool_false))) ->
   e' = s_expr_val (s_val_prim_c (s_prim_c_bool s_bool_true)) ->
-  (P, H, S, e) --> (P, H, S, e')
-| CStepNot3 : forall P H S e e' b σ,
+  (P, H, Σ, e) --> (P, H, Σ, e')
+| CStepNot3 : forall P H Σ e e' b σ,
   e = s_expr_not (s_expr_val σ) ->
   σ <> s_val_prim_c (s_prim_c_bool b) ->
   e' = s_expr_val (s_val_not σ) ->
-  (P, H, S, e) --> (P, H, S, e')
-| CStepEq1 : forall P H S e n1 n2 e',
+  (P, H, Σ, e) --> (P, H, Σ, e')
+| CStepEq1 : forall P H Σ e e' n1 n2,
   e = s_expr_eq (s_expr_val (s_val_prim_c (s_prim_c_int (s_int_l n1)))) (s_expr_val (s_val_prim_c (s_prim_c_int (s_int_l n2)))) ->
   e' = s_expr_val (s_val_prim_c (s_prim_c_bool (if Nat.eqb n1 n2 then s_bool_true else s_bool_false))) ->
-  (P, H, S, e) --> (P, H, S, e')
-| CStepEq2 : forall P H S e e',
+  (P, H, Σ, e) --> (P, H, Σ, e')
+| CStepEq2 : forall P H Σ e e',
   e = s_expr_eq (s_expr_val (s_val_prim_c (s_prim_c_bool s_bool_true))) (s_expr_val (s_val_prim_c (s_prim_c_bool s_bool_true))) ->
   e' = s_expr_val (s_val_prim_c (s_prim_c_bool s_bool_true)) ->
-  (P, H, S, e) --> (P, H, S, e')
-| CStepEq3 : forall P H S e e',
+  (P, H, Σ, e) --> (P, H, Σ, e')
+| CStepEq3 : forall P H Σ e e',
   e = s_expr_eq (s_expr_val (s_val_prim_c (s_prim_c_bool s_bool_false))) (s_expr_val (s_val_prim_c (s_prim_c_bool s_bool_false))) ->
   e' = s_expr_val (s_val_prim_c (s_prim_c_bool s_bool_true)) ->
-  (P, H, S, e) --> (P, H, S, e')
-| CStepEq4 : forall P H S e e',
+  (P, H, Σ, e) --> (P, H, Σ, e')
+| CStepEq4 : forall P H Σ e e',
   e = s_expr_eq (s_expr_val (s_val_prim_c (s_prim_c_bool s_bool_true))) (s_expr_val (s_val_prim_c (s_prim_c_bool s_bool_false))) ->
   e' = s_expr_val (s_val_prim_c (s_prim_c_bool s_bool_false)) ->
-  (P, H, S, e) --> (P, H, S, e')
-| CStepEq5 : forall P H S e e',
+  (P, H, Σ, e) --> (P, H, Σ, e')
+| CStepEq5 : forall P H Σ e e',
   e = s_expr_eq (s_expr_val (s_val_prim_c (s_prim_c_bool s_bool_false))) (s_expr_val (s_val_prim_c (s_prim_c_bool s_bool_true))) ->
   e' = s_expr_val (s_val_prim_c (s_prim_c_bool s_bool_false)) ->
-  (P, H, S, e) --> (P, H, S, e')
-| CStepEq6 : forall P H S e e',
+  (P, H, Σ, e) --> (P, H, Σ, e')
+| CStepEq6 : forall P H Σ e e',
   e = s_expr_eq (s_expr_val (s_val_ref_c s_ref_c_null)) (s_expr_val (s_val_ref_c s_ref_c_null)) ->
   e' = s_expr_val (s_val_prim_c (s_prim_c_bool s_bool_true)) ->
-  (P, H, S, e) --> (P, H, S, e')
-| CStepEq7 : forall P H S e e' l,
+  (P, H, Σ, e) --> (P, H, Σ, e')
+| CStepEq7 : forall P H Σ e e' l,
   e = s_expr_eq (s_expr_val (s_val_ref_c (s_ref_c_loc l))) (s_expr_val (s_val_ref_c s_ref_c_null)) ->
   e' = s_expr_val (s_val_prim_c (s_prim_c_bool s_bool_false)) ->
-  (P, H, S, e) --> (P, H, S, e')
-| CStepEq8 : forall P H S e e' l,
+  (P, H, Σ, e) --> (P, H, Σ, e')
+| CStepEq8 : forall P H Σ e e' l,
   e = s_expr_eq (s_expr_val (s_val_ref_c s_ref_c_null)) (s_expr_val (s_val_ref_c (s_ref_c_loc l))) ->
   e' = s_expr_val (s_val_prim_c (s_prim_c_bool s_bool_false)) ->
-  (P, H, S, e) --> (P, H, S, e')
-| CStepEq9 : forall P H S e e' n1 n2,
+  (P, H, Σ, e) --> (P, H, Σ, e')
+| CStepEq9 : forall P H Σ e e' n1 n2,
   e = s_expr_eq (s_expr_val (s_val_ref_c (s_ref_c_loc (s_loc_l n1)))) (s_expr_val (s_val_ref_c (s_ref_c_loc (s_loc_l n2)))) ->
   e' = s_expr_val (s_val_prim_c (s_prim_c_bool (if Nat.eqb n1 n2 then s_bool_true else s_bool_false))) ->
-  (P, H, S, e) --> (P, H, S, e')
-| CStepEq10 : forall P H S e e' l s,
+  (P, H, Σ, e) --> (P, H, Σ, e')
+| CStepEq10 : forall P H Σ e e' l s,
   e = s_expr_eq (s_expr_val (s_val_ref_c (s_ref_c_loc l))) (s_expr_val (s_val_ref_c (s_ref_c_symb s))) ->
   e' = s_expr_val (s_val_prim_c (s_prim_c_bool s_bool_false)) ->
-  (P, H, S, e) --> (P, H, S, e')
-| CStepEq11 : forall P H S e e' l s,
+  (P, H, Σ, e) --> (P, H, Σ, e')
+| CStepEq11 : forall P H Σ e e' l s,
   e = s_expr_eq (s_expr_val (s_val_ref_c (s_ref_c_symb s))) (s_expr_val (s_val_ref_c (s_ref_c_loc l))) ->
   e' = s_expr_val (s_val_prim_c (s_prim_c_bool s_bool_false)) ->
-  (P, H, S, e) --> (P, H, S, e')
-| CStepEq12 : forall P H S e e' l σ1 σ2 σ3,
+  (P, H, Σ, e) --> (P, H, Σ, e')
+| CStepEq12 : forall P H Σ e e' l σ1 σ2 σ3,
   e = s_expr_eq (s_expr_val (s_val_ref_c (s_ref_c_loc l))) (s_expr_val (s_val_ite σ1 σ2 σ3)) ->
   e' = s_expr_val (s_val_prim_c (s_prim_c_bool s_bool_false)) ->
-  (P, H, S, e) --> (P, H, S, e')
-| CStepEq13 : forall P H S e e' l σ1 σ2 σ3,
+  (P, H, Σ, e) --> (P, H, Σ, e')
+| CStepEq13 : forall P H Σ e e' l σ1 σ2 σ3,
   e = s_expr_eq (s_expr_val (s_val_ite σ1 σ2 σ3)) (s_expr_val (s_val_ref_c (s_ref_c_loc l))) ->
   e' = s_expr_val (s_val_prim_c (s_prim_c_bool s_bool_false)) ->
-  (P, H, S, e) --> (P, H, S, e')
-| CStepEq14 : forall P H S e e' n b l s σ1 σ2 σ3 σ4 σ5,
+  (P, H, Σ, e) --> (P, H, Σ, e')
+| CStepEq14 : forall P H Σ e e' n b l s σ1 σ2 σ3 σ4 σ5,
   e = s_expr_eq (s_expr_val σ1) (s_expr_val σ2) ->
   ((σ1 <> s_val_prim_c (s_prim_c_int (s_int_l n)) /\ σ1 <> s_val_prim_c (s_prim_c_bool b) /\
   σ1 <> s_val_ref_c s_ref_c_null /\ σ1 <> s_val_ref_c (s_ref_c_loc (s_loc_l n))) \/
@@ -366,51 +367,51 @@ Inductive cstep : config -> config -> Prop :=
   ~(σ1 = (s_val_ref_c (s_ref_c_loc l)) /\ σ2 = (s_val_ite σ3 σ4 σ5)) ->
   ~(σ2 = (s_val_ref_c (s_ref_c_loc l)) /\ σ1 = (s_val_ite σ3 σ4 σ5)) ->
   e' = s_expr_val (s_val_eq σ1 σ2) ->
-  (P, H, S, e) --> (P, H, S, e')
-| CStepInstanceof1 : forall P H S e e' c,
+  (P, H, Σ, e) --> (P, H, Σ, e')
+| CStepInstanceof1 : forall P H Σ e e' c,
   e = s_expr_instanceof (s_expr_val (s_val_ref_c s_ref_c_null)) c ->
   e' = s_expr_val (s_val_prim_c (s_prim_c_bool s_bool_false)) ->
-  (P, H, S, e) --> (P, H, S, e')
-| CStepInstanceof2 : forall P H S e e' l n c c',
+  (P, H, Σ, e) --> (P, H, Σ, e')
+| CStepInstanceof2 : forall P H Σ e e' l n c c',
   e = s_expr_instanceof (s_expr_val (s_val_ref_c l)) c ->
   l = s_ref_c_loc (s_loc_l n) ->
   obj_class_at H l = Some c' ->
   subclass P c' c ->
   e' = s_expr_val (s_val_prim_c (s_prim_c_bool s_bool_true)) ->
-  (P, H, S, e) --> (P, H, S, e')
-| CStepInstanceof3 : forall P H S e e' l n c c',
+  (P, H, Σ, e) --> (P, H, Σ, e')
+| CStepInstanceof3 : forall P H Σ e e' l n c c',
   e = s_expr_instanceof (s_expr_val (s_val_ref_c l)) c ->
   l = s_ref_c_loc (s_loc_l n) ->
   obj_class_at H l = Some c' ->
   ~(subclass P c' c) ->
   e' = s_expr_val (s_val_prim_c (s_prim_c_bool s_bool_false)) ->
-  (P, H, S, e) --> (P, H, S, e')
-| CStepInstanceof4 : forall P H S e e' Y s c,
+  (P, H, Σ, e) --> (P, H, Σ, e')
+| CStepInstanceof4 : forall P H Σ e e' Y s c,
   e = s_expr_instanceof (s_expr_val (s_val_ref_c Y)) c ->
   Y = s_ref_c_symb s ->
   e' = s_expr_val (s_val_subtype (s_val_ref_c Y) (s_ty_class c)) ->
-  (P, H, S, e) --> (P, H, S, e')
-| CStepInstanceof5 : forall P H S e σ c σ1 σ2 σ1' σ2' e',
-  (P, H, S, s_expr_instanceof (s_expr_val σ1) c) ==> (P, H, S, (s_expr_val σ1')) ->
-  (P, H, S, s_expr_instanceof (s_expr_val σ2) c) ==> (P, H, S, (s_expr_val σ2')) ->
+  (P, H, Σ, e) --> (P, H, Σ, e')
+| CStepInstanceof5 : forall P H Σ e e' σ c σ1 σ2 σ1' σ2',
+  (P, H, Σ, s_expr_instanceof (s_expr_val σ1) c) ==> (P, H, Σ, (s_expr_val σ1')) ->
+  (P, H, Σ, s_expr_instanceof (s_expr_val σ2) c) ==> (P, H, Σ, (s_expr_val σ2')) ->
   e = s_expr_instanceof (s_expr_val (s_val_ite σ σ1 σ2)) c ->
   e' = s_expr_val (s_val_ite σ σ1' σ2') ->
-  (P, H, S, e) --> (P, H, S, e')
-| CStepIf1 : forall P H S e e1 e2,
+  (P, H, Σ, e) --> (P, H, Σ, e')
+| CStepIf1 : forall P H Σ e e1 e2,
   e = s_expr_if (s_expr_val (s_val_prim_c (s_prim_c_bool s_bool_true))) e1 e2 ->
-  (P, H, S, e) --> (P, H, S, e1)
-| CStepIf2 : forall P H S e e1 e2,
+  (P, H, Σ, e) --> (P, H, Σ, e1)
+| CStepIf2 : forall P H Σ e e1 e2,
   e = s_expr_if (s_expr_val (s_val_prim_c (s_prim_c_bool s_bool_false))) e1 e2 ->
-  (P, H, S, e) --> (P, H, S, e2)
-| CStepIf3 : forall P H S e σ e1 e2 S',
+  (P, H, Σ, e) --> (P, H, Σ, e2)
+| CStepIf3 : forall P H Σ Σ' e e1 e2 σ,
   e = s_expr_if (s_expr_val σ) e1 e2 ->
-  S' = S ++ [σ] ->
-  (P, H, S, e) --> (P, H, S', e1)
-| CStepIf4 : forall P H S e σ e1 e2 S',
+  Σ' = Σ ++ [σ] ->
+  (P, H, Σ, e) --> (P, H, Σ', e1)
+| CStepIf4 : forall P H Σ Σ' e e1 e2 σ,
   e = s_expr_if (s_expr_val σ) e1 e2 ->
-  S' = S ++ [σ] ->
-  (P, H, S, e) --> (P, H, S', e2)
-| CStepInvoke1 : forall P H S e e' l n m σ o c c' t1 t2 xM eM,
+  Σ' = Σ ++ [s_val_not σ] ->
+  (P, H, Σ, e) --> (P, H, Σ', e2)
+| CStepInvoke1 : forall P H Σ e e' l n m σ o c c' t1 t2 xM eM,
   e = s_expr_invoke (s_expr_val (s_val_ref_c l)) m (s_expr_val σ) ->
   l = s_ref_c_loc (s_loc_l n) ->
   has_obj H l o ->
@@ -418,75 +419,75 @@ Inductive cstep : config -> config -> Prop :=
   recv_method P m c c' ->
   mdecl P c' m = Some (s_dc_m_l t1 m (s_dc_v_l t2 xM) eM) ->
   e' = repl_var (repl_var eM "this" (s_expr_val (s_val_ref_c l))) xM (s_expr_val σ) ->
-  (P, H, S, e) --> (P, H, S, e')
-| CStepInvoke2 : forall P H S e e' Y s m σ c' t1 t2 xM eM O cl1 cl2 S',
+  (P, H, Σ, e) --> (P, H, Σ, e')
+| CStepInvoke2 : forall P H Σ Σ' e e' eM Y s m σ c' t1 t2 xM O σ1' σ2',
   e = s_expr_invoke (s_expr_val (s_val_ref_c Y)) m (s_expr_val σ) ->
   Y = s_ref_c_symb s ->
   mdecl P c' m = Some (s_dc_m_l t1 m (s_dc_v_l t2 xM) eM) ->
   forall c, (In c O <-> overrides P m c c') ->
-  cl1 = s_val_not (s_val_eq (s_val_ref_c Y) (s_val_ref_c s_ref_c_null)) -> (* TODO redundant? *)
-  cl2 = s_val_subtype (s_val_ref_c Y) (s_ty_class c') ->
-  S' = S ++ [cl1 ; cl2] ++ map (fun c => s_val_not (s_val_subtype (s_val_ref_c Y) (s_ty_class c))) O ->
+  σ1' = s_val_not (s_val_eq (s_val_ref_c Y) (s_val_ref_c s_ref_c_null)) -> (* TODO redundant? *)
+  σ2' = s_val_subtype (s_val_ref_c Y) (s_ty_class c') ->
+  Σ' = Σ ++ [σ1' ; σ2'] ++ map (fun c => s_val_not (s_val_subtype (s_val_ref_c Y) (s_ty_class c))) O ->
   e' = repl_var (repl_var eM "this" (s_expr_val (s_val_ref_c Y))) xM (s_expr_val σ) ->
-  (P, H, S, e) --> (P, H, S', e')
-| CStepInvoke3 : forall P H S σ m e e1' σ1 σ2 σ' S1' S',
-  (P, H, S, s_expr_invoke (s_expr_val σ1) m (s_expr_val σ')) ==> (P, H, S1', e1') ->
+  (P, H, Σ, e) --> (P, H, Σ', e')
+| CStepInvoke3 : forall P H Σ Σ' Σ1' m e e1' σ σ' σ1 σ2,
+  (P, H, Σ, s_expr_invoke (s_expr_val σ1) m (s_expr_val σ')) ==> (P, H, Σ1', e1') ->
   e = s_expr_invoke (s_expr_val (s_val_ite σ σ1 σ2)) m (s_expr_val σ') ->
-  S' = S1' ++ [σ] ->
-  (P, H, S, e) --> (P, H, S', e1')
-| CStepInvoke4 : forall P H S σ m e e2' σ1 σ2 σ' S2' S',
-  (P, H, S, s_expr_invoke (s_expr_val σ2) m (s_expr_val σ')) ==> (P, H, S2', e2') ->
+  Σ' = Σ1' ++ [σ] ->
+  (P, H, Σ, e) --> (P, H, Σ', e1')
+| CStepInvoke4 : forall P H Σ Σ' Σ2' m e e2' σ σ' σ1 σ2,
+  (P, H, Σ, s_expr_invoke (s_expr_val σ2) m (s_expr_val σ')) ==> (P, H, Σ2', e2') ->
   e = s_expr_invoke (s_expr_val (s_val_ite σ σ1 σ2)) m (s_expr_val σ') ->
-  S' = S2' ++ [s_val_not σ] ->
-  (P, H, S, e) --> (P, H, S', e2')
-| CStepCtxGetfield : forall P H H' S S' e e' f,
-  (P, H, S, e) --> (P, H', S', e') ->  
-  (P, H, S, s_expr_getfield e f) --> (P, H', S', s_expr_getfield e' f)
-| CStepCtxPutfield1 : forall P H H' S S' e e' e1 f,
-  (P, H, S, e) --> (P, H', S', e') ->  
-  (P, H, S, s_expr_putfield e f e1) --> (P, H', S', s_expr_putfield e' f e1)
-| CStepCtxPutfield2 : forall P H H' S S' e e' σ f,
-  (P, H, S, e) --> (P, H', S', e') ->  
-  (P, H, S, s_expr_putfield (s_expr_val σ) f e) --> (P, H', S', s_expr_putfield (s_expr_val σ) f e')
-| CStepCtxLet : forall P H H' S S' e e' e1 x,
-  (P, H, S, e) --> (P, H', S', e') ->  
-  (P, H, S, s_expr_let x e e1) --> (P, H', S', s_expr_let x e' e1)
-| CStepCtxAdd1 : forall P H H' S S' e e' e1,
-  (P, H, S, e) --> (P, H', S', e') ->  
-  (P, H, S, s_expr_add e e1) --> (P, H', S', s_expr_add e' e1)
-| CStepCtxAdd2 : forall P H H' S S' e e' σ,
-  (P, H, S, e) --> (P, H', S', e') ->  
-  (P, H, S, s_expr_add (s_expr_val σ) e) --> (P, H', S', s_expr_add (s_expr_val σ) e')
-| CStepCtxSub1 : forall P H H' S S' e e' e1,
-  (P, H, S, e) --> (P, H', S', e') ->  
-  (P, H, S, s_expr_sub e e1) --> (P, H', S', s_expr_sub e' e1)
-| CStepCtxSub2 : forall P H H' S S' e e' σ,
-  (P, H, S, e) --> (P, H', S', e') ->  
-  (P, H, S, s_expr_sub (s_expr_val σ) e) --> (P, H', S', s_expr_sub (s_expr_val σ) e')
-| CStepCtxLt1 : forall P H H' S S' e e' e1,
-  (P, H, S, e) --> (P, H', S', e') ->
-  (P, H, S, s_expr_lt e e1) --> (P, H', S', s_expr_lt e' e1)
-| CStepCtxLt2 : forall P H H' S S' e e' σ,
-    (P, H, S, e) --> (P, H', S', e') ->
-  (P, H, S, s_expr_lt (s_expr_val σ) e) --> (P, H', S', s_expr_lt (s_expr_val σ) e')
-| CStepCtxEq1 : forall P H H' S S' e e' e1,
-  (P, H, S, e) --> (P, H', S', e') ->  
-  (P, H, S, s_expr_eq e e1) --> (P, H', S', s_expr_eq e' e1)
-| CStepCtxEq2 : forall P H H' S S' e e' σ,
-  (P, H, S, e) --> (P, H', S', e') ->  
-  (P, H, S, s_expr_eq (s_expr_val σ) e) --> (P, H', S', s_expr_eq (s_expr_val σ) e')
-| CStepCtxInstanceof : forall P H H' S S' e e' c,
-  (P, H, S, e) --> (P, H', S', e') ->  
-  (P, H, S, s_expr_instanceof e c) --> (P, H', S', s_expr_instanceof e' c)
-| CStepCtxIf : forall P H H' S S' e e' e1 e2,
-  (P, H, S, e) --> (P, H', S', e') ->  
-  (P, H, S, s_expr_if e e1 e2) --> (P, H', S', s_expr_if e' e1 e2)
-| CStepCtxInvoke1 : forall P H H' S S' e e' e1 m,
-  (P, H, S, e) --> (P, H', S', e') ->  
-  (P, H, S, s_expr_invoke e m e1) --> (P, H', S', s_expr_invoke e' m e1)
-| CStepCtxInvoke2 : forall P H H' S S' e e' σ m,
-  (P, H, S, e) --> (P, H', S', e') ->  
-  (P, H, S, s_expr_invoke (s_expr_val σ) m e) --> (P, H', S', s_expr_invoke (s_expr_val σ) m e')
+  Σ' = Σ2' ++ [s_val_not σ] ->
+  (P, H, Σ, e) --> (P, H, Σ', e2')
+| CStepCtxGetfield : forall P H H' Σ Σ' e e' f,
+  (P, H, Σ, e) --> (P, H', Σ', e') ->  
+  (P, H, Σ, s_expr_getfield e f) --> (P, H', Σ', s_expr_getfield e' f)
+| CStepCtxPutfield1 : forall P H H' Σ Σ' e e' e1 f,
+  (P, H, Σ, e) --> (P, H', Σ', e') ->  
+  (P, H, Σ, s_expr_putfield e f e1) --> (P, H', Σ', s_expr_putfield e' f e1)
+| CStepCtxPutfield2 : forall P H H' Σ Σ' e e' σ f,
+  (P, H, Σ, e) --> (P, H', Σ', e') ->  
+  (P, H, Σ, s_expr_putfield (s_expr_val σ) f e) --> (P, H', Σ', s_expr_putfield (s_expr_val σ) f e')
+| CStepCtxLet : forall P H H' Σ Σ' e e' e1 x,
+  (P, H, Σ, e) --> (P, H', Σ', e') ->  
+  (P, H, Σ, s_expr_let x e e1) --> (P, H', Σ', s_expr_let x e' e1)
+| CStepCtxAdd1 : forall P H H' Σ Σ' e e' e1,
+  (P, H, Σ, e) --> (P, H', Σ', e') ->  
+  (P, H, Σ, s_expr_add e e1) --> (P, H', Σ', s_expr_add e' e1)
+| CStepCtxAdd2 : forall P H H' Σ Σ' e e' σ,
+  (P, H, Σ, e) --> (P, H', Σ', e') ->  
+  (P, H, Σ, s_expr_add (s_expr_val σ) e) --> (P, H', Σ', s_expr_add (s_expr_val σ) e')
+| CStepCtxSub1 : forall P H H' Σ Σ' e e' e1,
+  (P, H, Σ, e) --> (P, H', Σ', e') ->  
+  (P, H, Σ, s_expr_sub e e1) --> (P, H', Σ', s_expr_sub e' e1)
+| CStepCtxSub2 : forall P H H' Σ Σ' e e' σ,
+  (P, H, Σ, e) --> (P, H', Σ', e') ->  
+  (P, H, Σ, s_expr_sub (s_expr_val σ) e) --> (P, H', Σ', s_expr_sub (s_expr_val σ) e')
+| CStepCtxLt1 : forall P H H' Σ Σ' e e' e1,
+  (P, H, Σ, e) --> (P, H', Σ', e') ->
+  (P, H, Σ, s_expr_lt e e1) --> (P, H', Σ', s_expr_lt e' e1)
+| CStepCtxLt2 : forall P H H' Σ Σ' e e' σ,
+  (P, H, Σ, e) --> (P, H', Σ', e') ->
+  (P, H, Σ, s_expr_lt (s_expr_val σ) e) --> (P, H', Σ', s_expr_lt (s_expr_val σ) e')
+| CStepCtxEq1 : forall P H H' Σ Σ' e e' e1,
+  (P, H, Σ, e) --> (P, H', Σ', e') ->  
+  (P, H, Σ, s_expr_eq e e1) --> (P, H', Σ', s_expr_eq e' e1)
+| CStepCtxEq2 : forall P H H' Σ Σ' e e' σ,
+  (P, H, Σ, e) --> (P, H', Σ', e') ->  
+  (P, H, Σ, s_expr_eq (s_expr_val σ) e) --> (P, H', Σ', s_expr_eq (s_expr_val σ) e')
+| CStepCtxInstanceof : forall P H H' Σ Σ' e e' c,
+  (P, H, Σ, e) --> (P, H', Σ', e') ->  
+  (P, H, Σ, s_expr_instanceof e c) --> (P, H', Σ', s_expr_instanceof e' c)
+| CStepCtxIf : forall P H H' Σ Σ' e e' e1 e2,
+  (P, H, Σ, e) --> (P, H', Σ', e') ->  
+  (P, H, Σ, s_expr_if e e1 e2) --> (P, H', Σ', s_expr_if e' e1 e2)
+| CStepCtxInvoke1 : forall P H H' Σ Σ' e e' e1 m,
+  (P, H, Σ, e) --> (P, H', Σ', e') ->  
+  (P, H, Σ, s_expr_invoke e m e1) --> (P, H', Σ', s_expr_invoke e' m e1)
+| CStepCtxInvoke2 : forall P H H' Σ Σ' e e' σ m,
+  (P, H, Σ, e) --> (P, H', Σ', e') ->  
+  (P, H, Σ, s_expr_invoke (s_expr_val σ) m e) --> (P, H', Σ', s_expr_invoke (s_expr_val σ) m e')
 with step : config -> config -> Prop :=
 | Step : forall J J' J'', J ~~>* J' -> J' --> J'' -> J ==> J''
 where " x '-->' y " := (cstep x y)
